add lemmas about hyper wp

Lgtm/HSepLog.lean
@@ -835,4 +835,130 @@ lemma htriple_ptr_add (v₁ : α -> loc) (v₂ : α -> Int) :
   sby move=> imp; apply htriple_prod_val_eq_emp=> ? /imp ?
       apply triple_ptr_add
 
-end end HTriple
+end
+end HTriple
+
+section HWeakestPrecondition
+
+open Classical trm val prim
+
+variable {α : Type} (s : Set α)
+
+local notation "htrm" => htrm α
+local notation "hval" => hval α
+local notation "hhProp" => hhProp α
+
+/- ---------- Definition and Structural Rules for [wp] ---------- -/
+
+/- Definition of [wp] -/
+
+
+def hwp (ht : htrm) (Q : hval -> hhProp) : hhProp := (heval s · ht Q)
+
+/- Equivalence b/w [wp] and [triple] -/
+
+lemma hwp_equiv : H ==> hwp s ht Q = htriple s ht H Q := by rfl
+
+/- Consequence rule for [wp] -/
+lemma hwp_conseq (ht : htrm) (Q Q' : hval -> hhProp) :
+  Q ===> Q' -> hwp s ht Q ==> hwp s ht Q' := by
+  sby move=> ???/=; apply heval_conseq
+
+/- Frame rule for [wp] -/
+
+lemma hwp_frame (ht : htrm) (Q : hval -> hhProp) (H : hhProp) :
+  hwp s ht Q ∗ H ==> hwp s ht (Q ∗ H) := by
+  move=> ? ![> ?? -> ?];
+  apply heval_conseq; apply heval_frame=> //
+  -- xsimp
+  sorry
+
+
+/- Corollaries -/
+
+lemma hwp_ramified :
+  (hwp s ht Q) ∗ (Q -∗ Q') ==> hwp s ht Q' := by
+  apply hhimpl_trans
+  { apply hwp_frame }
+  apply hwp_conseq
+  sby srw -hqwand_equiv
+
+lemma hwp_conseq_frame :
+  Q1 ∗ H ===> Q2 →
+  (hwp s t Q1) ∗ H ==> (hwp s t Q2) :=
+by
+  srw -hqwand_equiv
+  move=> M
+  apply @hhimpl_trans (h₂ := (hwp s t Q1) ∗ (Q1 -∗ Q2))
+  { sby apply hhimpl_frame_r }
+  apply hwp_ramified
+
+lemma hwp_ramified_trans t H Q1 Q2 :
+  H ==> (hwp s t Q1) ∗ (Q1 -∗ Q2) →
+  H ==> (hwp s t Q2) :=
+by
+  move=> M
+  -- xchange
+  sorry
+
+lemma hwp_union (s₁ s₂ : Set α) :
+  Disjoint s₁ s₂ ->
+  hwp (s₁ ∪ s₂) ht Q = hwp s₁ ht (fun hv => hwp s₂ ht (fun hv' => Q (hv ∪_s₁ hv'))) := by
+    move=> ?
+    apply hhimpl_antisymm=> ?<;> unfold hwp=> ?
+    { sby apply heval_unfocus }
+    sby apply heval_focus
+
+@[simp]
+lemma fun_insert0: (hv ∪_∅ hv') = hv' := by
+  sby funext a; simp [hunion, fun_insert]
+
+lemma hwp0_dep : hwp (∅ : Set α) ht Q = h∃ hv, Q hv := by
+  apply hhimpl_antisymm=> h <;> unfold hwp
+  { scase! => hQ _ /(_ (fun _ : α => val_unit)) /(_ h) H
+    specialize H ?_=> //
+    sby scase!: H=> hv' }
+  scase! => hv /= ?; exists (fun _ _ _ => True)=> ⟨?//|? h' heq ⟨//|⟩/==⟩
+  sby shave<-//: h = h'; funext x; move: (heq x)
+
+lemma hwp0 : hwp (∅ : Set α) ht (fun _ => Q) = Q := by
+  sby srw hwp0_dep; apply hhimpl_antisymm=> ?; scase!
+
+/- ---------- Hyper Weakest-Precondition Reasoning Rules for Hyper Terms ---------- -/
+
+lemma hwp_val v (Q : hval -> hhProp) :
+  Q v ==> hwp s (trm_val ∘ v) Q :=
+by sby apply htriple_val
+
+lemma hwp_fun (x : α -> var) (ht : α -> trm) (Q : hval -> hhProp) :
+  (Q fun a => val_fun (x a) (ht a)) ==> hwp s (fun a => trm_fun (x a) (ht a)) Q :=
+  by sby apply htriple_fun
+
+lemma hwp_fix (x f : α -> var) (ht : α -> trm) (Q : hval -> hhProp) :
+  (Q fun a => val_fix (f a) (x a) (ht a)) ==> hwp s (fun a => trm_fix (f a) (x a) (ht a)) Q :=
+  by sby apply htriple_fix
+
+lemma hwp_if (b : α -> Bool) (ht₁ ht₂ : α -> trm) (Q : hval -> hhProp) :
+  hwp s (fun a => if b a then ht₁ a else ht₂ a) Q ==> hwp s (fun a => trm_if (val_bool (b a)) (ht₁ a) (ht₂ a)) Q :=
+  by sby apply htriple_if
+
+lemma hwp_app_fun (hv₁ : hval) (x : α -> var) (ht₁ : α -> trm) (hv₂ : hval) (Q : hval -> hhProp) :
+  (forall d, d ∈ s -> hv₁ d = val_fun (x d) (ht₁ d)) ->
+  hwp s (fun a => subst (x a) (hv₂ a) (ht₁ a)) Q ==> hwp s (fun a => trm_app (hv₁ a) (hv₂ a)) Q :=
+  by sby move=> ?; apply htriple_app_fun
+
+lemma hwp_app_fix (hv₁ : hval) (x f : α -> var) (ht₁ : α -> trm) (hv₂ : hval) (Q : hval -> hhProp) :
+  (forall d, d ∈ s -> hv₁ d = val_fix (f d) (x d) (ht₁ d)) ->
+  hwp s (fun a => subst (x a) (hv₂ a) $ subst (f a) (hv₁ a) $ ht₁ a) Q ==> hwp s (fun a => trm_app (hv₁ a) (hv₂ a)) Q :=
+  by sby move=> ?; apply htriple_app_fix
+
+lemma hwp_seq (ht₁ ht₂ : htrm) (Q : hval -> hhProp) :
+  hwp s ht₁ (fun _ => hwp s ht₂ Q) ==> hwp s (fun a => trm_seq (ht₁ a) (ht₂ a)) Q :=
+  by sby move=> ??; apply heval_seq
+
+lemma hwp_let (x : α -> var) (ht₁ ht₂ : htrm) (Q : hval -> hhProp) :
+  hwp s ht₁ (fun v ↦ hwp s (fun a => subst (x a) (v a) (ht₂ a)) Q) ==> hwp s (fun a => trm_let (x a) (ht₁ a) (ht₂ a)) Q :=
+  by sby move=> ??; apply heval_let
+
+
+end HWeakestPrecondition
